Foundation/Vorspiel/Rel/WCWF.lean
@@ -1,0 +1,41 @@
+module
+
+public import Foundation.Vorspiel.Rel.CWF
+
+/-!
+# Weakly converse well-founded relations
+-/
+
+@[expose]
+public section
+
+/-- The irreflexive part of a relation. -/
+def Rel.IrreflGen {α} (r : Rel α α) : Rel α α := fun x y ↦ r x y ∧ x ≠ y
+
+@[simp, grind =]
+lemma Rel.irreflGen_iff {α} {r : Rel α α} {x y : α} : r.IrreflGen x y ↔ r x y ∧ x ≠ y := Iff.rfl
+
+abbrev WeaklyConverseWellFounded {α} (rel : Rel α α) := ConverseWellFounded rel.IrreflGen
+
+class IsWeaklyConverseWellFounded (α) (rel : Rel α α) : Prop where
+  wcwf : WeaklyConverseWellFounded rel
+
+section
+
+variable {α} {r : Rel α α}
+
+lemma WeaklyConverseWellFounded.has_max [IsWeaklyConverseWellFounded α r] (s : Set α)
+    (hs : s.Nonempty) : ∃ m ∈ s, ∀ x ∈ s, r m x → m = x := by
+  obtain ⟨m, hm, h⟩ := ConverseWellFounded.iff_has_max.mp (IsWeaklyConverseWellFounded.wcwf (rel := r)) s hs;
+  exact ⟨m, hm, fun x hx hmx ↦ by grind⟩;
+
+instance : Std.Irrefl r.IrreflGen := ⟨fun _ h ↦ h.2 rfl⟩
+
+instance [IsTrans α r] [Std.Antisymm r] : IsTrans α r.IrreflGen where
+  trans a b c hab hbc :=
+    ⟨IsTrans.trans a b c hab.1 hbc.1, by rintro rfl; exact hab.2 (Std.Antisymm.antisymm a b hab.1 hbc.1)⟩
+
+instance [Finite α] [IsTrans α r] [Std.Antisymm r] : IsWeaklyConverseWellFounded α r :=
+  ⟨Finite.converseWellFounded_of_trans_of_irrefl⟩
+
+end
